commit

AP/Defs.lean
@@ -3,13 +3,12 @@ import AP.Util
 noncomputable section
 open scoped Classical
 
-@[ext]
-structure Point where
-  x : ℤ
-  y : ℤ
+def Point := ℤ × ℤ
 
-def point₀ : Point := ⟨0, 0⟩
+@[simp] abbrev Point.x (p : Point) := p.1
+@[simp] abbrev Point.y (p : Point) := p.2
 
+def point₀ : Point := (0, 0)
 instance : Inhabited Point := ⟨point₀⟩
 
 def Point.dist (a b : Point) : ℕ :=
