AP/Strategy.lean
@@ -53,7 +53,7 @@ theorem state_push_state {st : State} {s} : (st.push s).toState' = s := rfl
 
 @[simp, symm]
 theorem point_dist_comm {a b : Point} : a.dist b = b.dist a := by
-  simp [Point.dist,abs_sub_comm]
+  simp [Point.dist, abs_sub_comm]
 
 theorem a_has_move_iff {s : State'} : s.a_has_move ↔ ∃ (p : Point),
 p ∈ s.grid ∧ p ≠ s.a_pos ∧ s.a_pos.dist p ≤ s.pw := by
@@ -70,55 +70,75 @@ theorem point_dist_eq_zero_iff {a b : Point} : a.dist b = 0 ↔ a = b := by
   have h₂ : |a.y - b.y| ≤ 0 := by apply (Int.le_neg_of_le_neg h).trans; simp
   simp [Int.sub_eq_zero] at h₁ h₂; ext <;> assumption
 
-theorem not_a_hws_0 : ¬a_hws 0 := by
-  unfold a_hws Game.a_wins; push_neg; intro a
-  use default, 2; simp [game₀_move]
-  generalize hm : (default : DStrat).1.f (state₀ 0) = m
+theorem game₀_0_play_2_ended {a d} : ((game₀ 0 a d).play 2).ended := by
+  simp [game₀_move]
+  generalize hm : d.1.f (state₀ 0) = m
   rcases m; simp at hm; nm s; simp
   suffices h : s.pw = 0 by simp [a_has_move_iff, h]
-  generalize (default : DStrat) = d at hm
   rcases d with ⟨⟨ms, f, h₁⟩, h₂⟩; dsimp at h₂ hm; subst h₂
   specialize h₁ # state₀ 0; simp [hm] at h₁
   obtain ⟨p, h₁, h₂⟩ := h₁; simp [h₁]
 
-def mk_a_strat' (f : State → Point) := λ (s : State) =>
-  let s' := {s with a_pos := f s}
-  if ¬s.a_has_move then none else some #
-  if s.a_move s' then s' else Classical.epsilon s.a_move
+theorem not_a_hws_0 : ¬a_hws 0 := by
+  unfold a_hws Game.a_wins; push_neg; intro a
+  use default, 2, game₀_0_play_2_ended
 
-def mk_a_strat (f : State → Point) : AStrat := by
-  refine' ⟨⟨_, mk_a_strat' f, _⟩, rfl⟩; intro s; dsimp; split
+@[simp]
+def mk_strat (m : State' → State' → Prop) (g : State' → Point → State')
+(f : State → Point) (s : State) :=
+  let s' := s.toState'
+  let s_new := g s' # f s
+  let fn := m s'
+  if ∀ s₁, ¬fn s₁ then none else some #
+  if fn s_new then s_new else Classical.epsilon fn
+
+def mk_a_strat' := mk_strat State'.a_move
+  λ s p => {s with a_pos := p}
+
+def mk_d_strat' := mk_strat State'.d_move
+  λ s p => {s with grid := s.grid.erase p}
+
+theorem mk_a_strat_valid {f : State → Point} {s : State} :
+let set := setOf λ (s₁ : State') =>
+  ∃ a₁, s₁ = { pw := s.pw, grid := s.grid, a_pos := a₁ } ∧
+  a₁ ∈ s.grid ∧ a₁ ≠ s.a_pos ∧ a₁.dist s.a_pos ≤ s.pw;
+match mk_a_strat' f s with
+| none => set = ∅
+| some s₁ => s₁ ∈ set := by
+  dsimp; split
   · nm m h; ext x; change (x ∈ setOf _) ↔ _
     simp only [Set.mem_setOf_eq, Set.mem_empty_iff_false,
       iff_false, not_exists, not_and, not_le]
     rintro p rfl h₁ h₂
-    simp only [mk_a_strat', a_has_move_iff, ne_eq, point_dist_comm,
-      not_exists, not_and, not_le, ite_eq_left_iff, not_forall,
-      Classical.not_imp, not_lt, reduceCtorEq, imp_false] at h
-    exact h _ h₁ h₂
-  · nm m s' h; change s' ∈ setOf _; simp only [Set.mem_setOf_eq]
-    use s'.a_pos; simp [mk_a_strat'] at h; obtain ⟨h₁, h₂⟩ := h
-    split_ifs at h₂ with h₃
-    · simp [←h₂]; simp [State'.a_move] at h₃; exact h₃
+    simp only [mk_a_strat'] at h; simp at h
+    simp only [State'.a_move, ne_eq, not_exists, not_and, not_le] at h
+    exact h _ p rfl h₁ h₂
+  · nm m s' h; use s'.a_pos; simp [mk_a_strat'] at h
+    obtain ⟨h₁, h₂⟩ := h; split_ifs at h₂ with h₃
+    · simp [←h₂]; simp only [State'.a_move, State'.mk.injEq,
+      implies_true, imp_self, true_and, ne_eq, exists_eq_left',
+      point_dist_comm] at h₃; exact h₃
     have h₄ := Classical.epsilon_spec h₁; rw [h₂] at h₄; clear h₂
     obtain ⟨a, rfl, h₄⟩ := h₄; simpa
 
-def mk_d_strat' (f : State → Point) := λ (s : State) =>
-  let s' := {s with grid := s.grid.erase # f s}
-  if ¬s.d_has_move then none else some #
-  if s.d_move s' then s' else Classical.epsilon s.d_move
-
-def mk_d_strat (f : State → Point) : DStrat := by
-  refine' ⟨⟨_, mk_d_strat' f, _⟩, rfl⟩; intro s; dsimp; split
+theorem mk_d_strat_valid {f : State → Point} {s : State} :
+let set := setOf λ (s₁ : State') =>
+  ∃ p, s₁ = { pw := s.pw, grid := Set.erase p s.grid, a_pos := s.a_pos } ∧
+  p ∈ s.grid ∧ p ≠ s.a_pos;
+match mk_d_strat' f s with
+| none => set = ∅
+| some s₁ => s₁ ∈ set := by
+  dsimp; split
   · nm m h; ext x; change (x ∈ setOf _) ↔ _
     simp only [Set.mem_setOf_eq, Set.mem_empty_iff_false, iff_false,
       not_exists, not_and, Decidable.not_not]; rintro p rfl h₁
-    simp only [mk_d_strat', State'.d_has_move, not_exists, ite_eq_left_iff,
-      not_forall, Decidable.not_not, reduceCtorEq, imp_false] at h
+    simp only [mk_d_strat'] at h; simp at h
+    simp only [State'.d_move, ne_eq, not_exists,
+      not_and, Decidable.not_not] at h
     specialize h {s with grid := s.grid.erase p}
     simp [State'.d_move] at h; apply h p rfl h₁
-  · nm m s' h; change s' ∈ setOf _; simp only [Set.mem_setOf_eq]
-    obtain ⟨p, hp⟩ := hv # Classical.epsilon λ p => p ∈ s.grid \ s'.grid
+  · nm m s' h; obtain ⟨p, hp⟩ := hv # Classical.epsilon
+      λ p => p ∈ s.grid \ s'.grid
     use p; simp [mk_d_strat'] at h; obtain ⟨h₁, h₂⟩ := h
     split_ifs at h₂ with h₃
     · simp [State'.d_move] at h₃; subst h₂; simp at hp ⊢
@@ -145,6 +165,12 @@ def mk_d_strat (f : State → Point) : DStrat := by
     simp only [State'.d_move, ←hg] at h₄
     obtain hp₁ := Classical.epsilon_spec h₄
     simp [←h₅] at hp; rw [←hp] at hp₁; simp [hg] at hp₁; exact hp₁
+
+def mk_a_strat (f : State → Point) : AStrat := by
+  refine' ⟨⟨_, mk_a_strat' f, _⟩, rfl⟩; apply mk_a_strat_valid
+
+def mk_d_strat (f : State → Point) : DStrat := by
+  refine' ⟨⟨_, mk_d_strat' f, _⟩, rfl⟩; apply mk_d_strat_valid
 
 @[simp]
 theorem not_state'₀_0_a_has_move : ¬(state'₀ 0).a_has_move := by
@@ -193,14 +219,163 @@ g.move.size = g.size + 1 := by
   have h₁ := game_not_ended_of_move_not_ended h; simp [Game.move, h₁]
   split; nm m h₂; contrapose! h; simp [Game.move, h₁, h₂]; simp
 
-#check 0 #exit
-
 theorem game_play_size_eq_of_not_ended {g : Game} {n} (h : ¬(g.play n).ended) :
 (g.play n).size = g.size + n := by
-  induction n
-  · simp
-  nm n ih
+  induction n; simp; nm n ih; simp at h ⊢
+  rw [game_move_size_eq_of_not_ended h,
+    ih # game_not_ended_of_move_not_ended h]; rfl
+
+theorem game_move_size_eq_of_ended {g : Game} (he : g.ended) :
+g.move.size = g.size := by simp [Game.move, he]
+
+theorem game_move_state_eq_of_move_ended {g : Game} (he : g.move.ended) :
+g.move.toState = g.toState := by
+  generalize hg₁ : g.move = g₁ at he ⊢
+  simp [Game.move] at hg₁; split_ifs at hg₁ with h₁ h₂; rw [hg₁]
+  all_goals split at hg₁ <;> subst hg₁ <;> first | rfl | contradiction
+
+theorem game_play_size_lt_iff_play_ended {g : Game} {n} (h₀ : ¬g.ended) :
+(g.play n).size < g.size + n ↔ (g.play n).ended := by
+  induction n; constructor <;> intro h <;> simp [h₀] at h
+  nm n ih; constructor <;> intro h
+  · simp at h ⊢; by_contra he₁
+    have he := game_not_ended_of_move_not_ended he₁; simp [he] at ih
+    rw [game_move_size_eq_of_not_ended he₁] at h; linarith
+  · simp at h ⊢; by_cases he : (g.play n).ended
+    · replace ih := ih.mpr he
+      suffices (g.play n).move.size = (g.play n).size by linarith
+      exact game_move_size_eq_of_ended he
+    suffices (g.play n).move.size = g.size + n by linarith
+    suffices (g.play n).move.size = (g.play n).size by
+      rw [this]; exact game_play_size_eq_of_not_ended he
+    rw [game_move_state_eq_of_move_ended h]
+
+@[simp]
+theorem state₀_size {pw} : (state₀ pw).size = 0 := rfl
+
+@[simp]
+theorem not_game₀_ended {pw a d} : ¬(game₀ pw a d).ended := λ h => h
+
+@[simp]
+theorem game_move_a_eq {g : Game} : g.move.a = g.a := by
+  rw [Game.move]; split_ifs <;> (try split) <;> rfl
+
+@[simp]
+theorem game_move_d_eq {g : Game} : g.move.d = g.d := by
+  rw [Game.move]; split_ifs <;> (try split) <;> rfl
+
+@[simp]
+theorem game_play_a_eq {g : Game} {n} : (g.play n).a = g.a := by
+  induction n <;> simp_all
+
+@[simp]
+theorem game_play_d_eq {g : Game} {n} : (g.play n).d = g.d := by
+  induction n <;> simp_all
+
+#check 0 #exit
+
+theorem exi_valid_state_with_size_of_pe_ne_0 {pw n}
+(h : pw ≠ 0) : ∃ (s : ValidState), s.pw = pw ∧ s.size = n := by
+  obtain ⟨fa, hfa⟩ := hv # λ (s : State) => (⟨s.size / 2 + 1, 0⟩ : Point)
+  obtain ⟨fd, hfd⟩ := hv # λ (s : State) => (⟨s.size / 2, 1⟩ : Point)
+  obtain ⟨a, ha⟩ := hv # mk_a_strat fa
+  obtain ⟨d, hd⟩ := hv # mk_d_strat fd
+  refine' ⟨⟨((game₀ pw a d).play n).toState, _⟩, _⟩
+  · apply state_valid_of_game_valid
+    simp
   simp
+  rw [game_play_size_eq_of_not_ended]; simp
+  apply and_intro # ((game₀ pw a d).play n).toState' =
+    { pw := pw
+    , grid := Set.univ \ {(x, y) | y = 1 ∧ 0 ≤ x ∧ x < (n + 1) / 2}
+    , a_pos := (n / 2, 0)
+    }
+  induction n
+  · simp only [game_play_zero, game₀_state, state₀_state, Nat.cast_zero,
+      zero_add, Int.reduceDiv, Int.zero_ediv, not_game₀_ended,
+      not_false_eq_true, implies_true, imp_self, and_true]
+    ext <;> try rfl
+    nm p
+    rcases p with ⟨x, y⟩
+    simp only [state'₀_grid, Set.mem_univ, implies_true, imp_self, Set.mem_diff,
+      Set.mem_setOf_eq, not_and, not_lt, and_self]
+  nm n ih
+  rcases ih with ⟨ih₁, ih₂⟩
+  rw [game_play_succ]
+  generalize hg : (game₀ pw a d).play n = g at *
+  have ⟨hga, hgd⟩ : g.a = a ∧ g.d = d := by simp [←hg]; exact ⟨rfl, rfl⟩
+  subst hga hgd
+  apply (by tauto : ∀ P Q, (Q → ¬P) → P → P ∧ ¬Q)
+  
+  · intro he
+    rw [game_move_state_eq_of_move_ended he, ih₁]
+    simp only [Nat.cast_add, Nat.cast_one, State'.mk.injEq, implies_true,
+      imp_self, point_mk_eq_iff, and_true, true_and, not_and]
+    clear * - n
+    intro h; contrapose! h
+    simp only [ne_eq, Set.ext_iff, Set.mem_diff, Set.mem_univ, implies_true,
+      imp_self, Set.mem_setOf_eq, true_and, not_forall]
+    have hn := Int.ofNat_zero_le n
+    generalize (n : ℤ) = n at *; nm x; clear x
+    rw [eq_comm] at h
+    use (n / 2, 1); simp
+    rw [int_succ_div_2_eq_div_iff hn] at h
+    rw [int_even_iff_exi] at h
+    obtain ⟨k, rfl⟩ := h
+    simp at hn
+    simp [hn]
+    rw [int_mul_2_succ_div_2_eq hn, add_assoc]
+    simp
+    rw [int_add_div_eq # by decide]
+    simp
+  
+  · simp [Game.move, ih₂]
+    split_ifs with ht
+    · have hn : Odd n := by sorry
+      
+      have h_a_move : g.a_move {g with a_pos := fa g.toState} := by
+        simp [hfa, ih₁, State'.a_move]
+        rw [←hg] at ih₂ ⊢
+        simp [game_play_size_eq_of_not_ended ih₂, Point.dist]
+        change 1 ≤ _
+        have h₁ : 0 ≤ (pw : ℤ) := by linarith
+        rw [le_iff_lt_or_eq] at h₁
+        rcases h₁ with h₁ | h₁
+        · linarith
+        contrapose! h
+        exact Int.ofNat_eq_zero.mp h₁.symm
+      
+      split
+      · nm m h₁
+        exfalso
+        simp at h₁
+        apply h₁; clear h₁
+        exact ⟨_, h_a_move⟩
+      · nm m s h₁
+        simp
+        simp [ha, mk_a_strat, mk_a_strat', h_a_move] at h₁
+        replace h₁ := h₁.2.symm
+        convert h₁ <;> clear h₁
+        · rw [←hg]; simp
+        · simp [ih₁]
+          congr
+          ext p
+          simp
+          rcases p with ⟨x, y⟩
+          simp
+          rintro rfl h₂
+          suffices ((n : ℤ) + 1 + 1) / 2 = ((n : ℤ) + 1) / 2 by rw [this]
+          rw [int_succ_div_2_eq_div_iff]
+          · simpa
+          linarith
+        · simp [hfa]
+          rw [game_play_size_eq_of_not_ended ih₂]
+
+#check 0 #exit
+
+theorem exi_valid_state_with_size_iff_pw_ne_0 {pw} :
+(∀ n, ∃ (s : ValidState), s.pw = pw ∧ s.size = n) ↔ pw ≠ 0 := by
+  constructor <;> intro h
 
 #check 0 #exit
 
