AP/Reachability.lean
@@ -3,7 +3,7 @@ import AP.Strategy
 noncomputable section
 open scoped Classical
 
-theorem card_grid_diff_le_1_of_subsingleton_pw_0_a_turn {g : Game} {n}
+theorem card_grid_diff_subsingleton_of_subsingleton_pw_0_a_turn {g : Game} {n}
 (h_pw : g.pw = 0) (h :  (Set.univ \ g.grid).Subsingleton)
 (ht : g.a_turn) : (Set.univ \ (g.play n).grid).Subsingleton := by
   unfold State'.grid at h ⊢; cases n; exact h; nm n; rw [game_play_succ']
@@ -14,18 +14,19 @@ theorem card_grid_diff_le_1_of_subsingleton_pw_0_a_turn {g : Game} {n}
   rwa [game_play_eq_of_ended h₁, ←State'.grid,
     game_move_grid_eq_of_move_ended h₁, State'.grid]
 
-theorem card_grid_diff_le_1_of_state'₀_0_a_turn {g : Game} {n}
+theorem card_grid_diff_subsingleton_of_state'₀_0_a_turn {g : Game} {n}
 (h :  g.toState' = state'₀ 0) (ht : g.a_turn) :
 (Set.univ \ (g.play n).grid).Subsingleton := by
-  apply card_grid_diff_le_1_of_subsingleton_pw_0_a_turn <;> simp [h, ht]
+  apply card_grid_diff_subsingleton_of_subsingleton_pw_0_a_turn <;>
+  simp [h, ht]
 
-theorem card_grid_diff_le_1_of_state'₀_0_not_a_turn {g : Game} {n}
+theorem card_grid_diff_subsingleton_of_state'₀_0_not_a_turn {g : Game} {n}
 (h :  g.toState' = state'₀ 0) (ht : ¬g.a_turn) :
 (Set.univ \ (g.play n).grid).Subsingleton := by
   by_cases he : g.ended
   · simp [Game.move, he, game_play_eq_of_ended he, h]
-  cases n; simp [h]; nm n
-  rw [game_play_succ']; apply card_grid_diff_le_1_of_subsingleton_pw_0_a_turn
+  cases n; simp [h]; nm n; rw [game_play_succ']
+  apply card_grid_diff_subsingleton_of_subsingleton_pw_0_a_turn
   · simp [h]
   · simp [Game.move, he, ht]; split; simp [h]
     nm m s h₁; simp; replace h₁ := of_d_ap_eq_some h₁
@@ -36,21 +37,19 @@ theorem card_grid_diff_le_1_of_state'₀_0_not_a_turn {g : Game} {n}
     apply d_always_has_move; simp [h]
   trivial
 
-theorem card_grid_diff_le_1_of_state'₀_0 {g : Game} {n}
+theorem card_grid_diff_subsingleton_of_state'₀_0 {g : Game} {n}
 (h :  g.toState' = state'₀ 0) :
 (Set.univ \ (g.play n).grid).Subsingleton := by
   by_cases h₁ : g.a_turn
-  exact card_grid_diff_le_1_of_state'₀_0_a_turn h h₁
-  exact card_grid_diff_le_1_of_state'₀_0_not_a_turn h h₁
+  exact card_grid_diff_subsingleton_of_state'₀_0_a_turn h h₁
+  exact card_grid_diff_subsingleton_of_state'₀_0_not_a_turn h h₁
 
 theorem not_Reachable'_imp_reachable :
 ¬(∀ (s₀ s : State'), s₀.Reachable' s → s₀.reachable s) := by
   push_neg; obtain ⟨s₁, hs₁⟩ := hv #
-    {state'₀ 0 with grid := Set.univ \
-    {(⟨0, 1⟩ : Point)}}
+    {state'₀ 0 with grid := Set.univ \ {(0, 1)}}
   obtain ⟨s₂, hs₂⟩ := hv #
-    {state'₀ 0 with grid := Set.univ \
-    {(⟨0, 1⟩ : Point), (⟨0, 2⟩ : Point)}}
+    {state'₀ 0 with grid := Set.univ \ {(0, 1), (0, 2)}}
   dsimp at hs₁ hs₂; use state'₀ 0, s₂
   constructor
   · apply State'.Reachable'.hd s₁
@@ -61,4 +60,4 @@ theorem not_Reachable'_imp_reachable :
   rw [eq_comm] at h₁; have h₂ := congrArg State'.grid hs₂
   dsimp at h₂; contrapose! h₂; clear h₂
   apply ne_of_congr λ s => (Set.univ \ s).Subsingleton
-  simp [h₁]; exact card_grid_diff_le_1_of_state'₀_0 h₁
+  simp [h₁]; exact card_grid_diff_subsingleton_of_state'₀_0 h₁
